First repair pass

src/lib/xmm_s_hb.v
@@ -8,6 +8,7 @@ From hahn Require Import Hahn.
 From imm Require Import Events.
 From imm Require Import Execution.
 From imm Require Import Execution_eco.
+From imm Require Import SubExecution.
 
 Set Implicit Arguments.
 
@@ -63,9 +64,9 @@ Implicit Type SC_PER_LOC : sc_per_loc G.
 (******************************************************************************)
 
 (* release sequence *)
-Definition rs := ⦗W⦘ ⨾ ⦗Rlx⦘ ⨾ (rf ⨾ rmw)＊.
+Definition rs := ⦗W⦘ ⨾ (rf ⨾ rmw)＊.
 
-Definition release := ⦗Rel⦘ ⨾ (⦗F⦘ ⨾ sb)^? ⨾ rs.
+Definition release := ⦗Rel⦘ ⨾ (⦗F⦘ ⨾ sb)^? ⨾ ⦗Rlx⦘ ⨾ rs.
 
 (* synchronizes with *)
 Definition sw := release ⨾ rf ⨾ ⦗Rlx⦘ ⨾ (sb ⨾ ⦗F⦘)^? ⨾ ⦗Acq⦘.
@@ -108,7 +109,7 @@ Proof using. destruct WF; unfold rs; desf; eauto 10 with hahn. Qed.
 (** ** Relations in graph *)
 (******************************************************************************)
 
-Lemma wf_rsE WF : rs ≡ ⦗W∩₁Rlx⦘ ∪ ⦗E⦘ ⨾ rs ⨾ ⦗E⦘.
+Lemma wf_rsE WF : rs ≡ ⦗W⦘ ∪ ⦗E⦘ ⨾ rs ⨾ ⦗E⦘.
 Proof using.
 unfold rs.
 split; [|basic_solver 15].
@@ -127,13 +128,15 @@ Qed.
 
 Lemma wf_releaseE WF : release ≡ ⦗W ∩₁ Rel⦘ ∪ ⦗E⦘ ⨾ release ⨾ ⦗E⦘.
 Proof using.
+arewrite (W ∩₁ Rel ≡₁ W ∩₁ Rel ∩₁ Rlx).
+{ rewrite set_interA. apply set_equiv_inter; [reflexivity |].
+  split; [| basic_solver]. unfolder.
+  unfold is_rel, is_rlx, mod, mode_le.
+  ins. desf. }
 unfold release.
 rewrite (wf_rsE WF).
 rewrite (@wf_sbE G) at 1.
 split; unfolder; ins; desf; eauto 42.
-eexists. splits; eauto.
-eexists. splits; eauto.
-mode_solver 42.
 Qed.
 
 Lemma wf_swE_right WF : sw ≡ sw ⨾ ⦗E⦘.
@@ -183,7 +186,7 @@ rewrite inclusion_ct_seq_eqv_r.
 basic_solver 42.
 Qed.
 
-Lemma wf_releaseD WF : release ≡ ⦗FW∩₁Rel⦘ ⨾ release ⨾ ⦗W⦘.
+Lemma wf_releaseD WF : release ≡ ⦗FW ∩₁ Rel⦘ ⨾ release ⨾ ⦗W⦘.
 Proof using.
 split; [|basic_solver].
 unfold release.
@@ -205,7 +208,7 @@ Qed.
 (** ** init *)
 (******************************************************************************)
 
-Lemma no_release_from_init WF: release ≡ ⦗set_compl is_init⦘ ⨾ release. 
+Lemma no_release_from_init WF: release ≡ ⦗set_compl is_init⦘ ⨾ release.
 Proof using.
   split; [| basic_solver]. apply doma_helper.
   unfold release. rewrite init_pln; eauto. mode_solver.
@@ -240,7 +243,7 @@ unfolder. ins. desf. eexists. splits; eauto.
 mode_solver.
 Qed.
 
-Lemma sw_in_release_rf WF: 
+Lemma sw_in_release_rf WF:
   sw ⨾ ⦗R⦘ ⊆ release ⨾ rf ⨾ ⦗Acq⦘.
 Proof using.
 unfold sw; rewrite !seqA.
@@ -251,7 +254,6 @@ Qed.
 Lemma rs_in_co WF SC_PER_LOC : rs ⊆ ⦗W⦘ ⨾ co^?.
 Proof using.
 unfold rs.
-arewrite_id ⦗Rlx⦘. rewrite seq_id_l.
 rewrite rtE; relsf; unionL; [basic_solver|].
 sin_rewrite !(rf_rmw_in_co WF SC_PER_LOC).
 sin_rewrite (dom_r (wf_coD WF)).
@@ -291,7 +293,7 @@ arewrite (sw ⊆ (sb ∪ sw)⁺) at 1; relsf.
 basic_solver 21.
 Qed.
 
-Lemma release_int : release ⊆ release ⨾ ⦗W_ex⦘ ∪ ⦗F ∩₁ Rel⦘ ⨾ sb ⨾ ⦗W⦘ ∪ 
+Lemma release_int : release ⊆ release ⨾ ⦗W_ex⦘ ∪ ⦗F ∩₁ Rel⦘ ⨾ sb ⨾ ⦗W⦘ ∪
   ⦗W ∩₁ Rel⦘ ⨾  (sb ∩ same_loc)^? ⨾ ⦗W⦘.
 Proof using.
 unfold release, rs.
@@ -326,8 +328,8 @@ Definition coherence := irreflexive (hb ⨾ eco^?).
 Implicit Type COH : coherence.
 
 Lemma coherence_sc_per_loc COH : sc_per_loc G.
-Proof using. 
-red; rewrite sb_in_hb. 
+Proof using.
+red; rewrite sb_in_hb.
 red in COH; unfolder in *; basic_solver 12.
 Qed.
 
@@ -350,3 +352,88 @@ all: try (unfolder in *; basic_solver 12).
 Qed.
 
 End IMM_hb.
+
+Section XMM_hb_sub.
+
+Variable G G' : execution.
+Variable sc sc' : relation actid.
+
+Notation "'lab''" := (lab G').
+Notation "'E''" := (acts_set G').
+Notation "'loc''" := (loc lab').
+Notation "'same_loc''" := (same_loc lab').
+Notation "'Acq''" := (fun e => is_true (is_acq lab' e)).
+Notation "'Rel''" := (fun e => is_true (is_rel lab' e)).
+Notation "'Rlx''" := (fun e => is_true (is_rlx lab' e)).
+Notation "'sb''" := (sb G').
+Notation "'rf''" := (rf G').
+Notation "'co''" := (co G').
+Notation "'rmw''" := (rmw G').
+Notation "'hb''" := (hb G').
+Notation "'rs''" := (rs G').
+Notation "'release''" := (release G').
+Notation "'sw''" := (sw G').
+Notation "'W''" := (fun e => is_true (is_w lab' e)).
+Notation "'R''" := (fun e => is_true (is_r lab' e)).
+Notation "'F''" := (fun e => is_true (is_f lab' e)).
+Notation "'Loc_'' l" := (fun x => loc' x = Some l) (at level 1).
+
+Notation "'lab'" := (lab G).
+Notation "'E'" := (acts_set G).
+Notation "'loc'" := (loc lab).
+Notation "'same_loc'" := (same_loc lab).
+Notation "'Acq'" := (fun e => is_true (is_acq lab e)).
+Notation "'Rel'" := (fun e => is_true (is_rel lab e)).
+Notation "'Rlx'" := (fun e => is_true (is_rlx lab e)).
+Notation "'sb'" := (sb G).
+Notation "'rf'" := (rf G).
+Notation "'co'" := (co G).
+Notation "'rmw'" := (rmw G).
+Notation "'hb'" := (hb G).
+Notation "'rs'" := (rs G).
+Notation "'release'" := (release G).
+Notation "'sw'" := (sw G).
+Notation "'W'" := (fun e => is_true (is_w lab e)).
+Notation "'R'" := (fun e => is_true (is_r lab e)).
+Notation "'F'" := (fun e => is_true (is_f lab e)).
+Notation "'Loc_' l" := (fun x => loc x = Some l) (at level 1).
+
+Hypothesis SUB : sub_execution G G' sc sc'.
+
+Lemma sub_rs_in : rs' ⊆ rs.
+Proof using SUB.
+  unfold rs.
+  now rewrite
+    (sub_lab SUB),
+    (sub_rf_in SUB),
+    (sub_rmw_in SUB).
+Qed.
+
+Lemma sub_release_in : release' ⊆ release.
+Proof using SUB.
+  unfold release.
+  now rewrite
+    (sub_lab SUB),
+    (sub_sb_in SUB),
+    sub_rs_in.
+Qed.
+
+Lemma sub_sw_in : sw' ⊆ sw.
+Proof using SUB.
+  unfold sw.
+  now rewrite
+    (sub_lab SUB),
+    (sub_rf_in SUB),
+    (sub_sb_in SUB),
+    sub_release_in.
+Qed.
+
+Lemma sub_hb_in : hb' ⊆ hb.
+Proof using SUB.
+  unfold hb.
+  now rewrite
+    (sub_sb_in SUB),
+    sub_sw_in.
+Qed.
+
+End XMM_hb_sub.
