src/lib/Rhb.v
@@ -1,0 +1,274 @@
+From hahn Require Import Hahn.
+From hahnExt Require Import HahnExt.
+From imm Require Import Events Execution.
+
+Require Import AuxRel.
+Require Import xmm_s_hb.
+
+Set Implicit Arguments.
+
+Section Rhb.
+Variable G : execution.
+Notation "'lab'" := (lab G).
+Notation "'E'" := (acts_set G).
+Notation "'loc'" := (loc lab).
+Notation "'same_loc'" := (same_loc lab).
+Notation "'Acq'" := (fun e => is_true (is_acq lab e)).
+Notation "'Rel'" := (fun e => is_true (is_rel lab e)).
+Notation "'Rlx'" := (fun e => is_true (is_rlx lab e)).
+Notation "'sb'" := (sb G).
+Notation "'rf'" := (rf G).
+Notation "'co'" := (co G).
+Notation "'rmw'" := (rmw G).
+Notation "'hb'" := (hb G).
+Notation "'sw'" := (sw G).
+Notation "'W'" := (fun e => is_true (is_w lab e)).
+Notation "'R'" := (fun e => is_true (is_r lab e)).
+Notation "'F'" := (fun e => is_true (is_f lab e)).
+Notation "'Loc_' l" := (fun x => loc x = Some l) (at level 1).
+
+Definition rpo_imm :=
+  ⦗R ∩₁ Rlx⦘ ⨾ sb ⨾ ⦗F ∩₁ Acq⦘ ∪
+  ⦗Acq⦘ ⨾ sb ∪
+  sb ⨾ ⦗Rel⦘ ∪
+  ⦗F ∩₁ Rel⦘ ⨾ sb ⨾ ⦗W ∩₁ Rlx⦘.
+Definition rpo := rpo_imm⁺.
+Definition rhb := (sb ∩ same_loc ∪ rpo ∪ sw)⁺.
+
+Lemma rpo_imm_in_sb : rpo_imm ⊆ sb.
+Proof using.
+  unfold rpo_imm.
+  basic_solver.
+Qed.
+
+Lemma rpo_in_sb : rpo ⊆ sb.
+Proof using.
+  unfold rpo. rewrite rpo_imm_in_sb.
+  apply ct_of_trans. apply sb_trans.
+Qed.
+
+Lemma wf_rpoE
+    (WF : Wf G) :
+  rpo ≡ ⦗E⦘ ⨾ rpo ⨾ ⦗E⦘.
+Proof using.
+  split; [| basic_solver].
+  unfolder. intros x y REL.
+  splits; ins.
+  all: apply rpo_in_sb in REL.
+  all: unfold sb in REL; unfolder in REL; desf.
+Qed.
+
+Lemma wf_rhbE
+    (WF : Wf G) :
+  rhb ≡ ⦗E⦘ ⨾ rhb ⨾ ⦗E⦘.
+Proof using.
+  apply dom_helper_3.
+  unfold rhb.
+  rewrite (wf_swE WF),
+          (wf_rpoE WF),
+          wf_sbE.
+  arewrite ((⦗E⦘ ⨾ sb ⨾ ⦗E⦘) ∩ same_loc ⊆ ⦗E⦘ ⨾ (sb ∩ same_loc) ⨾ ⦗E⦘).
+  { basic_solver. }
+  seq_rewrite <- !seq_union_r.
+  seq_rewrite <- !seq_union_l.
+  rewrite ct_seq_eqv_l.
+  rewrite <- seqA.
+  rewrite ct_seq_eqv_r.
+  basic_solver.
+Qed.
+
+Lemma rpo_imm_upward_closed s
+    (SBUP : upward_closed sb s) :
+  upward_closed rpo_imm s.
+Proof using.
+  unfold upward_closed, rpo_imm.
+  unfolder. intros x y HREL IN; desf.
+  all: eapply SBUP; eauto.
+Qed.
+
+Lemma rpo_upward_closed s
+    (SBUP : upward_closed sb s) :
+  upward_closed rpo s.
+Proof using.
+  unfold upward_closed, rpo.
+  intros x y REL.
+  apply clos_trans_tn1 in REL.
+  induction REL as [y REL | y z HEAD TAIL IHREL].
+  { intro HIN. eapply rpo_imm_upward_closed; eauto. }
+  intro HIN. apply IHREL.
+  eapply rpo_imm_upward_closed; eauto.
+Qed.
+
+Lemma rpo_to_rpo_imm a b
+    (SBIMM : immediate sb a b)
+    (RPO : rpo a b) :
+  rpo_imm a b.
+Proof using.
+  unfold rpo in RPO.
+  apply clos_trans_tn1 in RPO.
+  destruct RPO as [y RPO | y z HEAD TAIL]; ins.
+  apply clos_tn1_trans in TAIL.
+  apply rpo_in_sb in TAIL.
+  apply rpo_imm_in_sb in HEAD.
+  exfalso. now apply SBIMM with y.
+Qed.
+
+Lemma rpo_trans : transitive rpo.
+Proof using.
+  unfold rpo. apply transitive_ct.
+Qed.
+
+Lemma rhb_trans : transitive rhb.
+Proof using.
+  unfold rhb. apply transitive_ct.
+Qed.
+
+Lemma rhb_in_hb :
+    rhb ⊆ hb.
+Proof using.
+    unfold rhb; unfold hb.
+    apply clos_trans_mori.
+    rewrite rpo_in_sb; basic_solver.
+Qed.
+
+Lemma sb_sw_in_rpo_sw :
+    sb ⨾ sw ⊆ rpo ⨾ sw.
+Proof using.
+  transitivity (sb ⨾ ⦗Rel⦘ ⨾ sw).
+  { arewrite (sw ⊆ (⦗Rel⦘) ⨾ sw) at 1; [|done].
+    unfold sw. unfold release. basic_solver 42. }
+  hahn_frame_r.
+  unfold rpo, rpo_imm. rewrite <- ct_step.
+  eauto with hahn.
+Qed.
+
+Lemma sw_sb_in_rpo :
+    sw ⨾ sb ⊆ sw ⨾ rpo.
+Proof using.
+  transitivity (sw ⨾ ⦗Acq⦘ ⨾ sb).
+  { arewrite (sw ⊆ sw ;; (⦗Acq⦘)) at 1; [|done].
+    unfold sw. basic_solver 21. }
+  hahn_frame_l.
+  unfold rpo, rpo_imm. rewrite <- ct_step.
+  eauto with hahn.
+Qed.
+
+Lemma sb_sw_trans_in_rpo_sw_trans :
+    sb ⨾ sw⁺ ⊆ rpo ⨾ sw⁺.
+Proof using.
+  now rewrite ct_begin, <- !seqA, sb_sw_in_rpo_sw.
+Qed.
+
+Lemma sb_sw_trans_trans :
+    (sb ⨾ sw⁺)⁺ ⊆ (rpo ⨾ sw⁺)⁺.
+Proof using.
+  now rewrite sb_sw_trans_in_rpo_sw_trans.
+Qed.
+
+(* TODO: remove *)
+Lemma sb_rpo_start x x0 y
+        (SB : sb x x0)
+        (SW : sw x0 y) :
+    rpo x x0.
+Proof using.
+    unfold rpo. left. left. right. destruct SW. destruct H.
+    unfold release in H. assert (REL : is_rel lab x0).
+    { destruct H. destruct H. destruct H. basic_solver. }
+    basic_solver.
+Qed.
+
+Lemma rpo_sb_end x x0 y
+        (RPO : sw x x0)
+        (SB : sb x0 y) :
+    rpo x0 y.
+Proof using.
+    unfold rpo. left. left. left. right. destruct RPO. destruct H.
+    assert (ACQ : is_acq lab x0).
+    { destruct H0. destruct H0. destruct H1. destruct H1.
+      destruct H2. destruct H2. destruct H3. basic_solver. }
+    basic_solver.
+Qed.
+
+Lemma rpo_in_rhb :
+  rpo ⊆ rhb.
+Proof using.
+  unfold rhb. auto with hahn.
+Qed.
+
+Lemma sw_in_rhb :
+  sw ⊆ rhb.
+Proof using.
+  unfold rhb. auto with hahn.
+Qed.
+
+Lemma sb_loc_in_rhb :
+  sb ∩ same_loc ⊆ rhb.
+Proof using.
+  unfold rhb. auto with hahn.
+Qed.
+
+Lemma hb_helper :
+    hb ≡ sb ∪ rhb.
+Proof using.
+  split; [| rewrite rhb_in_hb, sb_in_hb; auto with hahn].
+  unfold hb, rhb. intros x y HH. apply clos_trans_t1n in HH.
+  assert (IN : sw＊ ⨾ (rpo ⨾ sw＊)⁺ ⊆ sw＊ ⨾ ((sb ∩ same_loc ∪ rpo) ⨾ sw＊)⁺).
+  { apply inclusion_seq_mon; [basic_solver |].
+    apply inclusion_t_t. apply inclusion_seq_mon; basic_solver. }
+  induction HH as [x y START | x y z STEP1 STEP2 IHSTEP].
+  { destruct START as [P1 | P2]; try basic_solver.
+    right. apply ct_step. basic_solver. }
+  destruct STEP1 as [P1 | P2]; destruct IHSTEP as [P3 | P4].
+  { left. assert (TRANS : transitive sb). apply sb_trans.
+    unfold transitive in TRANS. basic_solver. }
+  { assert (TRANS : transitive sb) by apply sb_trans.
+    rewrite <- clos_trans_t1n_iff in STEP2.
+    assert (PATH : (sb ⨾ (sb ∪ sw)⁺) x z) by basic_solver.
+    apply trans_helper in PATH; eauto.
+    destruct PATH as [PATH1 | PATH2]; [left; basic_solver |].
+    destruct PATH2 as (x0 & (PTH1 & [EQ | NEQ])). 2 :
+    { apply sb_sw_trans_trans in PTH1. assert (PTH1' := PTH1).
+      apply ct_end in PTH1. destruct PTH1 as (x1 & PTH1 & (x2 & PTH2 & PTH3)).
+      apply ct_end in PTH3. destruct PTH3 as (x3 & PTH3 & PTH4).
+      assert (RPO : rpo x0 z).
+      { apply rpo_sb_end with (x0 := x0) (x := x3); eauto. }
+      right. apply ct_ct. unfold seq. exists x0. split.
+      { apply ct_unionE. right. apply IN.
+        unfold seq. exists x. split; vauto.
+        assert (EQ : (fun x4 y0 : actid =>
+              exists z0 : actid, rpo x4 z0 /\ sw＊ z0 y0)⁺ ≡ (rpo ⨾ sw＊)⁺).
+        { unfold seq. basic_solver. }
+        apply EQ.
+        apply inclusion_t_t with (r := rpo ⨾ sw⁺); vauto.
+        apply inclusion_seq_mon; vauto.
+        apply inclusion_t_rt. }
+      apply ct_step. basic_solver. }
+    destruct EQ. apply sb_sw_trans_trans in PTH1. assert (PTH1' := PTH1).
+    right. apply ct_unionE. right. apply IN. unfold seq. exists x. split; vauto.
+    assert (EQ : (fun x4 y0 : actid =>
+          exists z0 : actid, rpo x4 z0 /\ sw＊ z0 y0)⁺ ≡ (rpo ⨾ sw＊)⁺).
+    { unfold seq. basic_solver. }
+    apply EQ.
+    apply inclusion_t_t with (r := rpo ⨾ sw⁺); basic_solver. }
+  { enough (RR : sw x y /\ rpo y z).
+    { right.
+      apply rhb_trans with y.
+      all: try now apply sw_in_rhb, RR.
+      all: try now apply rpo_in_rhb, RR. }
+    split; auto.
+    apply rpo_sb_end with (x := x); eauto. }
+  right. apply rhb_trans with y; auto.
+  now apply sw_in_rhb.
+Qed.
+
+Lemma hb_locs :
+    hb ∩ same_loc ≡ rhb ∩ same_loc.
+Proof using.
+    rewrite hb_helper; eauto; split.
+    2: { basic_solver. }
+    rewrite inter_union_l. rewrite inclusion_union_l with (r := sb ∩ same_loc)
+        (r' := rhb ∩ same_loc) (r'' := rhb ∩ same_loc); try basic_solver.
+    unfold rhb. rewrite <- ct_step. unfold rpo. basic_solver 8.
+Qed.
+
+End Rhb.
